@prefix : <http://www.bemserver.org/sensor/xssn/#> .
@prefix owl: <http://www.w3.org/2002/07/owl#> .
@prefix rdf: <http://www.w3.org/1999/02/22-rdf-syntax-ns#> .
@prefix ssn: <http://www.w3.org/ns/ssn/> .
@prefix xml: <http://www.w3.org/XML/1998/namespace> .
@prefix xsd: <http://www.w3.org/2001/XMLSchema#> .
@prefix rdfs: <http://www.w3.org/2000/01/rdf-schema#> .
@prefix sosa: <http://www.w3.org/ns/sosa/> .
@prefix xssn: <http://www.bemserver.org/sensor/xssn/#> .
@base <http://www.bemserver.org/sensor/xssn/#> .

<http://www.bemserver.org/sensor/xssn/#> rdf:type owl:Ontology ;
                                          owl:imports ssn: ;
                                          rdfs:comment "This ontology is based on the SSN ontology to model sensors, observations, features of intereset, etc. and extends it towards representing a location of a sensor or a location of an observation made by the sensor,  observation properties, and medium types on which the measurements are performed. It also introduces a new concept xssn:Property, which generalizes ssn:Property to further represent a wider set of properties including physical and occupant properties." .

#################################################################
#    Datatypes
#################################################################

###  http://www.bemserver.org/sensor/xssn/#ObservationMethod
xssn:ObservationMethod rdf:type rdfs:Datatype ;
                       owl:equivalentClass [ rdf:type rdfs:Datatype ;
                                             owl:oneOf [ rdf:type rdf:List ;
                                                         rdf:first "AT_FREQUENCY" ;
                                                         rdf:rest [ rdf:type rdf:List ;
                                                                    rdf:first "ON_CHANGE" ;
                                                                    rdf:rest rdf:nil
                                                                  ]
                                                       ]
                                           ] .


#################################################################
#    Object Properties
#################################################################

###  http://www.bemserver.org/sensor/xssn/#hasMedium
xssn:hasMedium rdf:type owl:ObjectProperty .


###  http://www.bemserver.org/sensor/xssn/#isLocatedIn
xssn:isLocatedIn rdf:type owl:ObjectProperty .


#################################################################
#    Data properties
#################################################################

###  http://www.bemserver.org/sensor/xssn/#accuracy
xssn:accuracy rdf:type owl:DatatypeProperty ;
              rdfs:comment "Accuracy represnts the closeness of agreement between the value of an observation and the true value of the observed quality."@en ;
              rdfs:seeAlso "http://www.w3.org/ns/ssn/systems/Accuracy" .


###  http://www.bemserver.org/sensor/xssn/#frequency
xssn:frequency rdf:type owl:DatatypeProperty ;
               rdfs:comment "Frequency represents the frequency of an observation capture in ms."@en ;
               rdfs:seeAlso "http://www.w3.org/ns/ssn/systems/Frequency" .


###  http://www.bemserver.org/sensor/xssn/#isAmbient
xssn:isAmbient rdf:type owl:DatatypeProperty ;
               rdfs:comment "isAmbient indicates whether the measure is an ambient one or not. For instance, a sensor measurement performed on the temperature in ome room/area of a building. Set points and measures made on HVAC equipment must not be ambient."@en .


###  http://www.bemserver.org/sensor/xssn/#isIndexValue
xssn:isIndexValue rdf:type owl:DatatypeProperty ;
                  rdfs:comment "isIndexValue indicates whether the measure is made on an index. In this case, values are cumulative."@en .


###  http://www.bemserver.org/sensor/xssn/#isSetPoint
xssn:isSetPoint rdf:type owl:DatatypeProperty ;
                rdfs:comment "isSetPoint indicates whether the measure is a set point."@en .


###  http://www.bemserver.org/sensor/xssn/#latency
xssn:latency rdf:type owl:DatatypeProperty ;
             rdfs:comment "Latency represents the time (in ms) between a request for an observation and the sensor providing a result."@en ;
             rdfs:seeAlso "http://www.w3.org/ns/ssn/systems/Latency" .


###  http://www.bemserver.org/sensor/xssn/#maxValue
xssn:maxValue rdf:type owl:DatatypeProperty ;
              rdfs:comment "minValue represents the maximum value accepted by the sensor"@en .


###  http://www.bemserver.org/sensor/xssn/#minValue
xssn:minValue rdf:type owl:DatatypeProperty ;
              rdfs:comment "minValue represents the minimum value accepted by the sensor"@en .


###  http://www.bemserver.org/sensor/xssn/#precision
xssn:precision rdf:type owl:DatatypeProperty ;
               rdfs:comment "Precision represents the closeness of agreement between replicate observations on an unchanged or similar quality value: i.e., a measure of a sensor's ability to consitently reproduce an observation."@en ;
               rdfs:seeAlso "IRI: http://www.w3.org/ns/ssn/systems/Precision" .


###  http://www.bemserver.org/sensor/xssn/#sensitivity
xssn:sensitivity rdf:type owl:DatatypeProperty ;
                 rdfs:comment "Sensitivity represents the quotient of the change in a result of sensor and the corresponding change in a value of a quality being observed."@en ;
                 rdfs:seeAlso "http://www.w3.org/ns/ssn/systems/Sensitivity" .


#################################################################
#    Classes
#################################################################

###  http://www.bemserver.org/sensor/xssn/#Location
xssn:Location rdf:type owl:Class ;
              rdfs:comment "Location represents the location of an observation or the location of a sensor. More details on Location can be represented through alignements with other ontologies such as xBOT"@en .


###  http://www.bemserver.org/sensor/xssn/#MediumType
xssn:MediumType rdf:type owl:Class ;
                owl:equivalentClass [ rdf:type owl:Class ;
                                      owl:oneOf ( xssn:AIR
                                                  xssn:GAS
                                                  xssn:OIL
                                                  xssn:RADIATION
                                                  xssn:STEAM
                                                  xssn:WATER
                                                )
                                    ] ;
                rdfs:comment "The physical medium on which the measure is performed.This is to be read in conjunction with the observation type. For instance an ambient air temperature sensor would have observation:type = Temperature and medium = Air."@en .


###  http://www.bemserver.org/sensor/xssn/#Property
xssn:Property rdf:type owl:Class ;
              rdfs:comment "A quality of an entity. An aspect of an entity that can be intrinsic to and cannot exist without the entity (such as sensors and devices) or can be optional for some entities (such building elements)."@en ;
              rdfs:label "Property"@en .


###  http://www.w3.org/ns/sosa/Observation
sosa:Observation rdfs:subClassOf [ rdf:type owl:Restriction ;
                                   owl:onProperty xssn:hasMedium ;
                                   owl:allValuesFrom xssn:MediumType
                                 ] ,
                                 [ rdf:type owl:Restriction ;
                                   owl:onProperty xssn:isLocatedIn ;
                                   owl:allValuesFrom xssn:Location
                                 ] ,
                                 [ rdf:type owl:Restriction ;
                                   owl:onProperty xssn:accuracy ;
                                   owl:allValuesFrom xsd:decimal
                                 ] ,
                                 [ rdf:type owl:Restriction ;
                                   owl:onProperty xssn:frequency ;
                                   owl:allValuesFrom xsd:decimal
                                 ] ,
                                 [ rdf:type owl:Restriction ;
                                   owl:onProperty xssn:latency ;
                                   owl:allValuesFrom xsd:integer
                                 ] ,
                                 [ rdf:type owl:Restriction ;
                                   owl:onProperty xssn:precision ;
                                   owl:allValuesFrom xsd:decimal
                                 ] ,
                                 [ rdf:type owl:Restriction ;
                                   owl:onProperty xssn:sensitivity ;
                                   owl:allValuesFrom xsd:decimal
                                 ] ,
                                 [ rdf:type owl:Restriction ;
                                   owl:onProperty xssn:isAmbient ;
                                   owl:qualifiedCardinality "1"^^xsd:nonNegativeInteger ;
                                   owl:onDataRange xsd:boolean
                                 ] ,
                                 [ rdf:type owl:Restriction ;
                                   owl:onProperty xssn:isIndexValue ;
                                   owl:qualifiedCardinality "1"^^xsd:nonNegativeInteger ;
                                   owl:onDataRange xsd:boolean
                                 ] ,
                                 [ rdf:type owl:Restriction ;
                                   owl:onProperty xssn:isSetPoint ;
                                   owl:qualifiedCardinality "1"^^xsd:nonNegativeInteger ;
                                   owl:onDataRange xsd:boolean
                                 ] ,
                                 [ rdf:type owl:Restriction ;
                                   owl:onProperty xssn:maxValue ;
                                   owl:qualifiedCardinality "1"^^xsd:nonNegativeInteger ;
                                   owl:onDataRange xsd:decimal
                                 ] ,
                                 [ rdf:type owl:Restriction ;
                                   owl:onProperty xssn:minValue ;
                                   owl:qualifiedCardinality "1"^^xsd:nonNegativeInteger ;
                                   owl:onDataRange xsd:decimal
                                 ] .


###  http://www.w3.org/ns/sosa/Sensor
sosa:Sensor rdfs:subClassOf [ rdf:type owl:Restriction ;
                              owl:onProperty xssn:isLocatedIn ;
                              owl:allValuesFrom xssn:Location
                            ] .


###  http://www.w3.org/ns/ssn/Property
ssn:Property rdfs:subClassOf xssn:Property .


#################################################################
#    Individuals
#################################################################

###  http://www.bemserver.org/sensor/xssn/#AIR
xssn:AIR rdf:type owl:NamedIndividual .


###  http://www.bemserver.org/sensor/xssn/#AT_FREQUENCY
xssn:AT_FREQUENCY rdf:type owl:NamedIndividual .


###  http://www.bemserver.org/sensor/xssn/#GAS
xssn:GAS rdf:type owl:NamedIndividual .


###  http://www.bemserver.org/sensor/xssn/#OIL
xssn:OIL rdf:type owl:NamedIndividual .


###  http://www.bemserver.org/sensor/xssn/#ON_VALUE_CHANGE
xssn:ON_VALUE_CHANGE rdf:type owl:NamedIndividual .


###  http://www.bemserver.org/sensor/xssn/#OTHER
xssn:OTHER rdf:type owl:NamedIndividual .


###  http://www.bemserver.org/sensor/xssn/#RADIATION
xssn:RADIATION rdf:type owl:NamedIndividual .


###  http://www.bemserver.org/sensor/xssn/#STEAM
xssn:STEAM rdf:type owl:NamedIndividual .


###  http://www.bemserver.org/sensor/xssn/#WATER
xssn:WATER rdf:type owl:NamedIndividual .


###  Generated by the OWL API (version 4.5.9.2019-02-01T07:24:44Z) https://github.com/owlcs/owlapi
