@prefix : <http://www.bemserver.org/sensor/xssn/#> .
@prefix owl: <http://www.w3.org/2002/07/owl#> .
@prefix rdf: <http://www.w3.org/1999/02/22-rdf-syntax-ns#> .
@prefix xml: <http://www.w3.org/XML/1998/namespace> .
@prefix xsd: <http://www.w3.org/2001/XMLSchema#> .
@prefix rdfs: <http://www.w3.org/2000/01/rdf-schema#> .
@base <http://www.bemserver.org/sensor/xssn/#> .

<http://www.bemserver.org/sensor/xssn/#> rdf:type owl:Ontology ;
                                          owl:imports <http://www.w3.org/ns/ssn/> ;
                                          rdfs:comment "This ontology is based on the SSN ontology to model sensors, observations, features of intereset, etc. and extends it towards representing a location of a sensor or a location of an observation made by the sensor,  observation properties, and medium types on which the measurements are performed. It also introduces a new concept xssn:Property, which generalizes ssn:Property to further represent a wider set of properties including physical and occupant properties." .

#################################################################
#    Annotation properties
#################################################################

###  http://purl.org/dc/terms/created
<http://purl.org/dc/terms/created> rdf:type owl:AnnotationProperty .


###  http://purl.org/dc/terms/creator
<http://purl.org/dc/terms/creator> rdf:type owl:AnnotationProperty .


###  http://purl.org/dc/terms/description
<http://purl.org/dc/terms/description> rdf:type owl:AnnotationProperty .


###  http://purl.org/dc/terms/license
<http://purl.org/dc/terms/license> rdf:type owl:AnnotationProperty .


###  http://purl.org/dc/terms/rights
<http://purl.org/dc/terms/rights> rdf:type owl:AnnotationProperty .


###  http://purl.org/dc/terms/title
<http://purl.org/dc/terms/title> rdf:type owl:AnnotationProperty .


###  http://purl.org/vocab/vann/preferredNamespacePrefix
<http://purl.org/vocab/vann/preferredNamespacePrefix> rdf:type owl:AnnotationProperty .


###  http://purl.org/vocab/vann/preferredNamespaceUri
<http://purl.org/vocab/vann/preferredNamespaceUri> rdf:type owl:AnnotationProperty .


###  http://www.w3.org/2004/02/skos/core#definition
<http://www.w3.org/2004/02/skos/core#definition> rdf:type owl:AnnotationProperty .


###  http://www.w3.org/2004/02/skos/core#example
<http://www.w3.org/2004/02/skos/core#example> rdf:type owl:AnnotationProperty .


###  http://xmlns.com/foaf/0.1/name
<http://xmlns.com/foaf/0.1/name> rdf:type owl:AnnotationProperty .


#################################################################
#    Datatypes
#################################################################

###  http://www.bemserver.org/sensor/xssn/#ObservationMethod
:ObservationMethod rdf:type rdfs:Datatype ;
                   owl:equivalentClass [ rdf:type rdfs:Datatype ;
                                         owl:oneOf [ rdf:type rdf:List ;
                                                     rdf:first "AT_FREQUENCY" ;
                                                     rdf:rest [ rdf:type rdf:List ;
                                                                rdf:first "ON_CHANGE" ;
                                                                rdf:rest rdf:nil
                                                              ]
                                                   ]
                                       ] .


#################################################################
#    Object Properties
#################################################################

###  http://www.bemserver.org/sensor/xssn/#hasMedium
:hasMedium rdf:type owl:ObjectProperty .


###  http://www.bemserver.org/sensor/xssn/#isLocatedIn
:isLocatedIn rdf:type owl:ObjectProperty .


###  http://www.w3.org/ns/sosa/actsOnProperty
<http://www.w3.org/ns/sosa/actsOnProperty> rdfs:isDefinedBy <http://www.w3.org/ns/sosa/> .


###  http://www.w3.org/ns/sosa/hasFeatureOfInterest
<http://www.w3.org/ns/sosa/hasFeatureOfInterest> rdfs:isDefinedBy <http://www.w3.org/ns/sosa/> .


###  http://www.w3.org/ns/sosa/hasResult
<http://www.w3.org/ns/sosa/hasResult> rdfs:isDefinedBy <http://www.w3.org/ns/sosa/> .


###  http://www.w3.org/ns/sosa/hasSample
<http://www.w3.org/ns/sosa/hasSample> rdf:type owl:ObjectProperty ,
                                               owl:InverseFunctionalProperty ;
                                      rdfs:isDefinedBy <http://www.w3.org/ns/sosa/> .


###  http://www.w3.org/ns/sosa/hosts
<http://www.w3.org/ns/sosa/hosts> owl:propertyChainAxiom ( <http://www.w3.org/ns/ssn/inDeployment>
                                                           <http://www.w3.org/ns/ssn/deployedSystem>
                                                         ) ;
                                  rdfs:isDefinedBy <http://www.w3.org/ns/sosa/> .


###  http://www.w3.org/ns/sosa/isActedOnBy
<http://www.w3.org/ns/sosa/isActedOnBy> rdfs:isDefinedBy <http://www.w3.org/ns/sosa/> .


###  http://www.w3.org/ns/sosa/isHostedBy
<http://www.w3.org/ns/sosa/isHostedBy> rdfs:isDefinedBy <http://www.w3.org/ns/sosa/> .


###  http://www.w3.org/ns/sosa/isObservedBy
<http://www.w3.org/ns/sosa/isObservedBy> rdfs:isDefinedBy <http://www.w3.org/ns/sosa/> .


###  http://www.w3.org/ns/sosa/isResultOf
<http://www.w3.org/ns/sosa/isResultOf> rdfs:isDefinedBy <http://www.w3.org/ns/sosa/> .


###  http://www.w3.org/ns/sosa/isSampleOf
<http://www.w3.org/ns/sosa/isSampleOf> rdf:type owl:FunctionalProperty ;
                                       rdfs:isDefinedBy <http://www.w3.org/ns/sosa/> .


###  http://www.w3.org/ns/sosa/madeActuation
<http://www.w3.org/ns/sosa/madeActuation> rdfs:isDefinedBy <http://www.w3.org/ns/sosa/> .


###  http://www.w3.org/ns/sosa/madeByActuator
<http://www.w3.org/ns/sosa/madeByActuator> rdfs:isDefinedBy <http://www.w3.org/ns/sosa/> .


###  http://www.w3.org/ns/sosa/madeBySampler
<http://www.w3.org/ns/sosa/madeBySampler> rdfs:isDefinedBy <http://www.w3.org/ns/sosa/> .


###  http://www.w3.org/ns/sosa/madeBySensor
<http://www.w3.org/ns/sosa/madeBySensor> rdfs:isDefinedBy <http://www.w3.org/ns/sosa/> .


###  http://www.w3.org/ns/sosa/madeObservation
<http://www.w3.org/ns/sosa/madeObservation> rdfs:isDefinedBy <http://www.w3.org/ns/sosa/> .


###  http://www.w3.org/ns/sosa/madeSampling
<http://www.w3.org/ns/sosa/madeSampling> rdfs:isDefinedBy <http://www.w3.org/ns/sosa/> .


###  http://www.w3.org/ns/sosa/observedProperty
<http://www.w3.org/ns/sosa/observedProperty> rdfs:isDefinedBy <http://www.w3.org/ns/sosa/> .


###  http://www.w3.org/ns/sosa/observes
<http://www.w3.org/ns/sosa/observes> rdfs:subPropertyOf <http://www.w3.org/ns/ssn/forProperty> ;
                                     rdfs:isDefinedBy <http://www.w3.org/ns/sosa/> .


###  http://www.w3.org/ns/sosa/phenomenonTime
<http://www.w3.org/ns/sosa/phenomenonTime> rdfs:isDefinedBy <http://www.w3.org/ns/sosa/> .


###  http://www.w3.org/ns/sosa/usedProcedure
<http://www.w3.org/ns/sosa/usedProcedure> owl:propertyChainAxiom ( <http://www.w3.org/ns/sosa/madeByActuator>
                                                                   <http://www.w3.org/ns/ssn/implements>
                                                                 ) ,
                                                                 ( <http://www.w3.org/ns/sosa/madeBySampler>
                                                                   <http://www.w3.org/ns/ssn/implements>
                                                                 ) ,
                                                                 ( <http://www.w3.org/ns/sosa/madeBySensor>
                                                                   <http://www.w3.org/ns/ssn/implements>
                                                                 ) ;
                                          rdfs:isDefinedBy <http://www.w3.org/ns/sosa/> .


###  http://www.w3.org/ns/ssn/deployedOnPlatform
<http://www.w3.org/ns/ssn/deployedOnPlatform> rdf:type owl:ObjectProperty ;
                                              owl:inverseOf <http://www.w3.org/ns/ssn/inDeployment> ;
                                              rdfs:comment "Relation between a Deployment and the Platform on which the Systems are deployed."@en ;
                                              rdfs:isDefinedBy <http://www.w3.org/ns/ssn/> ;
                                              rdfs:label "deployed on platform"@en ;
                                              <http://www.w3.org/2004/02/skos/core#definition> "Relation between a Deployment and the Platform on which the Systems are deployed."@en .


###  http://www.w3.org/ns/ssn/deployedSystem
<http://www.w3.org/ns/ssn/deployedSystem> rdf:type owl:ObjectProperty ;
                                          owl:inverseOf <http://www.w3.org/ns/ssn/hasDeployment> ;
                                          rdfs:comment "Relation between a Deployment and a deployed System."@en ;
                                          rdfs:isDefinedBy <http://www.w3.org/ns/ssn/> ;
                                          rdfs:label "deployed system"@en ;
                                          <http://www.w3.org/2004/02/skos/core#definition> "Relation between a Deployment and a deployed System."@en .


###  http://www.w3.org/ns/ssn/detects
<http://www.w3.org/ns/ssn/detects> rdf:type owl:ObjectProperty ;
                                   rdfs:comment "A relation from a Sensor to the Stimulus that the Sensor detects. The Stimulus itself will be serving as a proxy for some ObservableProperty."@en ;
                                   rdfs:isDefinedBy <http://www.w3.org/ns/ssn/> ;
                                   rdfs:label "detects"@en ;
                                   <http://www.w3.org/2004/02/skos/core#definition> "A relation from a Sensor to the Stimulus that the Sensor detects. The Stimulus itself will be serving as a proxy for some ObservableProperty."@en .


###  http://www.w3.org/ns/ssn/forProperty
<http://www.w3.org/ns/ssn/forProperty> rdf:type owl:ObjectProperty ;
                                       rdfs:comment "A relation between some aspect of an entity and a Property."@en ;
                                       rdfs:isDefinedBy <http://www.w3.org/ns/ssn/> ;
                                       rdfs:label "for property"@en ;
                                       <http://www.w3.org/2004/02/skos/core#definition> "A relation between some aspect of an entity and a Property."@en ;
                                       <http://www.w3.org/2004/02/skos/core#example> "For example, from a Sensor to the properties it can observe; from an Actuator to the properties it can act on; from a Deployment to the properties it was installed to observe or act on; from a SystemCapability to the Property the capability is described for."@en .


###  http://www.w3.org/ns/ssn/hasDeployment
<http://www.w3.org/ns/ssn/hasDeployment> rdf:type owl:ObjectProperty ;
                                         rdfs:comment "Relation between a System and a Deployment, recording that the System is deployed in that Deployment."@en ;
                                         rdfs:isDefinedBy <http://www.w3.org/ns/ssn/> ;
                                         rdfs:label "has deployment"@en ;
                                         <http://www.w3.org/2004/02/skos/core#definition> "Relation between a System and a Deployment, recording that the System is deployed in that Deployment."@en .


###  http://www.w3.org/ns/ssn/hasInput
<http://www.w3.org/ns/ssn/hasInput> rdf:type owl:ObjectProperty ;
                                    rdfs:comment "Relation between a Procedure and an Input to it."@en ;
                                    rdfs:isDefinedBy <http://www.w3.org/ns/ssn/> ;
                                    rdfs:label "has input"@en ;
                                    <http://www.w3.org/2004/02/skos/core#definition> "Relation between a Procedure and an Input to it."@en .


###  http://www.w3.org/ns/ssn/hasOutput
<http://www.w3.org/ns/ssn/hasOutput> rdf:type owl:ObjectProperty ;
                                     rdfs:comment "Relation between a Procedure and an Output of it."@en ;
                                     rdfs:isDefinedBy <http://www.w3.org/ns/ssn/> ;
                                     rdfs:label "has output"@en ;
                                     <http://www.w3.org/2004/02/skos/core#definition> "Relation between a Procedure and an Output of it."@en .


###  http://www.w3.org/ns/ssn/hasProperty
<http://www.w3.org/ns/ssn/hasProperty> rdf:type owl:ObjectProperty ;
                                       owl:inverseOf <http://www.w3.org/ns/ssn/isPropertyOf> ;
                                       rdfs:comment "Relation between an entity and a Property of that entity."@en ;
                                       rdfs:isDefinedBy <http://www.w3.org/ns/ssn/> ;
                                       rdfs:label "has property"@en ;
                                       <http://www.w3.org/2004/02/skos/core#definition> "Relation between an entity and a Property of that entity."@en .


###  http://www.w3.org/ns/ssn/hasSubSystem
<http://www.w3.org/ns/ssn/hasSubSystem> rdf:type owl:ObjectProperty ;
                                        rdfs:comment "Relation between a System and its component parts."@en ;
                                        rdfs:isDefinedBy <http://www.w3.org/ns/ssn/> ;
                                        rdfs:label "has subsystem"@en ;
                                        <http://www.w3.org/2004/02/skos/core#definition> "Relation between a System and its component parts."@en .


###  http://www.w3.org/ns/ssn/implementedBy
<http://www.w3.org/ns/ssn/implementedBy> rdf:type owl:ObjectProperty ;
                                         owl:inverseOf <http://www.w3.org/ns/ssn/implements> ;
                                         rdfs:comment "Relation between a Procedure (an algorithm, procedure or method) and an entity that implements that Procedure in some executable way."@en ;
                                         rdfs:isDefinedBy <http://www.w3.org/ns/ssn/> ;
                                         rdfs:label "implemented by"@en ;
                                         <http://www.w3.org/2004/02/skos/core#definition> "Relation between a Procedure (an algorithm, procedure or method) and an entity that implements that Procedure in some executable way."@en ;
                                         <http://www.w3.org/2004/02/skos/core#example> "For example, the relationship between a scientific measuring Procedure and a sensor that senses via that Procedure."@en .


###  http://www.w3.org/ns/ssn/implements
<http://www.w3.org/ns/ssn/implements> rdf:type owl:ObjectProperty ;
                                      rdfs:comment "Relation between an entity that implements a Procedure in some executable way and the Procedure (an algorithm, procedure or method)."@en ;
                                      rdfs:isDefinedBy <http://www.w3.org/ns/ssn/> ;
                                      rdfs:label "implements"@en ;
                                      <http://www.w3.org/2004/02/skos/core#definition> "Relation between an entity that implements a Procedure in some executable way and the Procedure (an algorithm, procedure or method)."@en ;
                                      <http://www.w3.org/2004/02/skos/core#example> "For example, the relationship between a sensor and the scientific measuring Procedure via which it senses."@en .


###  http://www.w3.org/ns/ssn/inDeployment
<http://www.w3.org/ns/ssn/inDeployment> rdf:type owl:ObjectProperty ;
                                        rdfs:comment "Relation between a Platform and a Deployment, meaning that the deployedSystems of the Deployment are hosted on the Platform."@en ;
                                        rdfs:isDefinedBy <http://www.w3.org/ns/ssn/> ;
                                        rdfs:label "in deployment"@en ;
                                        <http://www.w3.org/2004/02/skos/core#definition> "Relation between a Platform and a Deployment, meaning that the deployedSystems of the Deployment are hosted on the Platform."@en ;
                                        <http://www.w3.org/2004/02/skos/core#example> "For example, a relation between a buoy and a deployment of several Sensors."@en .


###  http://www.w3.org/ns/ssn/isPropertyOf
<http://www.w3.org/ns/ssn/isPropertyOf> rdf:type owl:ObjectProperty ;
                                        rdfs:comment "Relation between a Property and the entity it belongs to."@en ;
                                        rdfs:isDefinedBy <http://www.w3.org/ns/ssn/> ;
                                        rdfs:label "is property of"@en ;
                                        <http://www.w3.org/2004/02/skos/core#definition> "Relation between a Property and the entity it belongs to."@en .


###  http://www.w3.org/ns/ssn/isProxyFor
<http://www.w3.org/ns/ssn/isProxyFor> rdf:type owl:ObjectProperty ;
                                      rdfs:comment "A relation from a Stimulus to the Property that the Stimulus is serving as a proxy for."@en ;
                                      rdfs:isDefinedBy <http://www.w3.org/ns/ssn/> ;
                                      rdfs:label "is proxy for"@en ;
                                      <http://www.w3.org/2004/02/skos/core#definition> "A relation from a Stimulus to the Property that the Stimulus is serving as a proxy for."@en ;
                                      <http://www.w3.org/2004/02/skos/core#example> "For example, the expansion of quicksilver is a stimulus that serves as a proxy for some temperature property. An increase or decrease in the velocity of spinning cups on a wind sensor is serving as a proxy for the wind speed."@en .


###  http://www.w3.org/ns/ssn/wasOriginatedBy
<http://www.w3.org/ns/ssn/wasOriginatedBy> rdf:type owl:ObjectProperty ,
                                                    owl:FunctionalProperty ;
                                           rdfs:comment "Relation between an Observation and the Stimulus that originated it."@en ;
                                           rdfs:isDefinedBy <http://www.w3.org/ns/ssn/> ;
                                           rdfs:label "was originated by"@en ;
                                           <http://www.w3.org/2004/02/skos/core#definition> "Relation between an Observation and the Stimulus that originated it."@en .


#################################################################
#    Data properties
#################################################################

###  http://www.bemserver.org/sensor/xssn/#accuracy
:accuracy rdf:type owl:DatatypeProperty ;
          rdfs:comment "Accuracy represnts the closeness of agreement between the value of an observation and the true value of the observed quality."@en ;
          rdfs:seeAlso "http://www.w3.org/ns/ssn/systems/Accuracy" .


###  http://www.bemserver.org/sensor/xssn/#frequency
:frequency rdf:type owl:DatatypeProperty ;
           rdfs:comment "Frequency represents the frequency of an observation capture in ms."@en ;
           rdfs:seeAlso "http://www.w3.org/ns/ssn/systems/Frequency" .


###  http://www.bemserver.org/sensor/xssn/#isAmbient
:isAmbient rdf:type owl:DatatypeProperty ;
           rdfs:comment "isAmbient indicates whether the measure is an ambient one or not. For instance, a sensor measurement performed on the temperature in ome room/area of a building. Set points and measures made on HVAC equipment must not be ambient."@en .


###  http://www.bemserver.org/sensor/xssn/#isIndexValue
:isIndexValue rdf:type owl:DatatypeProperty ;
              rdfs:comment "isIndexValue indicates whether the measure is made on an index. In this case, values are cumulative."@en .


###  http://www.bemserver.org/sensor/xssn/#isSetPoint
:isSetPoint rdf:type owl:DatatypeProperty ;
            rdfs:comment "isSetPoint indicates whether the measure is a set point."@en .


###  http://www.bemserver.org/sensor/xssn/#latency
:latency rdf:type owl:DatatypeProperty ;
         rdfs:comment "Latency represents the time (in ms) between a request for an observation and the sensor providing a result."@en ;
         rdfs:seeAlso "http://www.w3.org/ns/ssn/systems/Latency" .


###  http://www.bemserver.org/sensor/xssn/#maxValue
:maxValue rdf:type owl:DatatypeProperty ;
          rdfs:comment "minValue represents the maximum value accepted by the sensor"@en .


###  http://www.bemserver.org/sensor/xssn/#minValue
:minValue rdf:type owl:DatatypeProperty ;
          rdfs:comment "minValue represents the minimum value accepted by the sensor"@en .


###  http://www.bemserver.org/sensor/xssn/#precision
:precision rdf:type owl:DatatypeProperty ;
           rdfs:comment "Precision represents the closeness of agreement between replicate observations on an unchanged or similar quality value: i.e., a measure of a sensor's ability to consitently reproduce an observation."@en ;
           rdfs:seeAlso "IRI: http://www.w3.org/ns/ssn/systems/Precision" .


###  http://www.bemserver.org/sensor/xssn/#sensitivity
:sensitivity rdf:type owl:DatatypeProperty ;
             rdfs:comment "Sensitivity represents the quotient of the change in a result of sensor and the corresponding change in a value of a quality being observed."@en ;
             rdfs:seeAlso "http://www.w3.org/ns/ssn/systems/Sensitivity" .


###  http://www.w3.org/ns/sosa/resultTime
<http://www.w3.org/ns/sosa/resultTime> rdfs:isDefinedBy <http://www.w3.org/ns/sosa/> .


#################################################################
#    Classes
#################################################################

###  http://purl.org/vocommons/voaf#Vocabulary
<http://purl.org/vocommons/voaf#Vocabulary> rdf:type owl:Class .


###  http://www.bemserver.org/sensor/xssn/#Location
:Location rdf:type owl:Class ;
          rdfs:comment "Location represents the location of an observation or the location of a sensor. More details on Location can be represented through alignements with other ontologies such as xBOT"@en .


###  http://www.bemserver.org/sensor/xssn/#MediumType
:MediumType rdf:type owl:Class ;
            owl:equivalentClass [ rdf:type owl:Class ;
                                  owl:oneOf ( :AIR
                                              :GAS
                                              :OIL
                                              :RADIATION
                                              :STEAM
                                              :WATER
                                            )
                                ] ;
            rdfs:comment "The physical medium on which the measure is performed.This is to be read in conjunction with the observation type. For instance an ambient air temperature sensor would have observation:type = Temperature and medium = Air."@en .


###  http://www.bemserver.org/sensor/xssn/#Property
:Property rdf:type owl:Class ;
          rdfs:comment "A quality of an entity. An aspect of an entity that can be intrinsic to and cannot exist without the entity (such as sensors and devices) or can be optional for some entities (such building elements)."@en ;
          rdfs:label "Property"@en .


###  http://www.w3.org/ns/sosa/ActuatableProperty
<http://www.w3.org/ns/sosa/ActuatableProperty> rdfs:subClassOf <http://www.w3.org/ns/ssn/Property> ,
                                                               [ rdf:type owl:Restriction ;
                                                                 owl:onProperty <http://www.w3.org/ns/sosa/isActedOnBy> ;
                                                                 owl:allValuesFrom <http://www.w3.org/ns/sosa/Actuation>
                                                               ] ;
                                               rdfs:isDefinedBy <http://www.w3.org/ns/sosa/> .


###  http://www.w3.org/ns/sosa/Actuation
<http://www.w3.org/ns/sosa/Actuation> rdf:type owl:Class ;
                                      rdfs:subClassOf [ rdf:type owl:Restriction ;
                                                        owl:onProperty <http://www.w3.org/ns/sosa/actsOnProperty> ;
                                                        owl:allValuesFrom <http://www.w3.org/ns/sosa/ActuatableProperty>
                                                      ] ,
                                                      [ rdf:type owl:Restriction ;
                                                        owl:onProperty <http://www.w3.org/ns/sosa/hasFeatureOfInterest> ;
                                                        owl:allValuesFrom <http://www.w3.org/ns/sosa/FeatureOfInterest>
                                                      ] ,
                                                      [ rdf:type owl:Restriction ;
                                                        owl:onProperty <http://www.w3.org/ns/sosa/hasResult> ;
                                                        owl:allValuesFrom <http://www.w3.org/ns/sosa/Result>
                                                      ] ,
                                                      [ rdf:type owl:Restriction ;
                                                        owl:onProperty <http://www.w3.org/ns/sosa/madeByActuator> ;
                                                        owl:allValuesFrom <http://www.w3.org/ns/sosa/Actuator>
                                                      ] ,
                                                      [ rdf:type owl:Restriction ;
                                                        owl:onProperty <http://www.w3.org/ns/sosa/usedProcedure> ;
                                                        owl:allValuesFrom <http://www.w3.org/ns/sosa/Procedure>
                                                      ] ,
                                                      [ rdf:type owl:Restriction ;
                                                        owl:onProperty <http://www.w3.org/ns/sosa/actsOnProperty> ;
                                                        owl:minCardinality "1"^^xsd:nonNegativeInteger
                                                      ] ,
                                                      [ rdf:type owl:Restriction ;
                                                        owl:onProperty <http://www.w3.org/ns/sosa/hasResult> ;
                                                        owl:minCardinality "1"^^xsd:nonNegativeInteger
                                                      ] ,
                                                      [ rdf:type owl:Restriction ;
                                                        owl:onProperty <http://www.w3.org/ns/sosa/hasFeatureOfInterest> ;
                                                        owl:cardinality "1"^^xsd:nonNegativeInteger
                                                      ] ,
                                                      [ rdf:type owl:Restriction ;
                                                        owl:onProperty <http://www.w3.org/ns/sosa/madeByActuator> ;
                                                        owl:cardinality "1"^^xsd:nonNegativeInteger
                                                      ] ,
                                                      [ rdf:type owl:Restriction ;
                                                        owl:onProperty <http://www.w3.org/ns/sosa/resultTime> ;
                                                        owl:cardinality "1"^^xsd:nonNegativeInteger
                                                      ] ;
                                      rdfs:isDefinedBy <http://www.w3.org/ns/sosa/> .


###  http://www.w3.org/ns/sosa/Actuator
<http://www.w3.org/ns/sosa/Actuator> rdfs:subClassOf <http://www.w3.org/ns/ssn/System> ,
                                                     [ rdf:type owl:Restriction ;
                                                       owl:onProperty <http://www.w3.org/ns/sosa/madeActuation> ;
                                                       owl:allValuesFrom <http://www.w3.org/ns/sosa/Actuation>
                                                     ] ,
                                                     [ rdf:type owl:Restriction ;
                                                       owl:onProperty <http://www.w3.org/ns/ssn/forProperty> ;
                                                       owl:allValuesFrom <http://www.w3.org/ns/sosa/ActuatableProperty>
                                                     ] ,
                                                     [ rdf:type owl:Restriction ;
                                                       owl:onProperty <http://www.w3.org/ns/ssn/implements> ;
                                                       owl:minCardinality "1"^^xsd:nonNegativeInteger
                                                     ] ;
                                     rdfs:isDefinedBy <http://www.w3.org/ns/sosa/> .


###  http://www.w3.org/ns/sosa/FeatureOfInterest
<http://www.w3.org/ns/sosa/FeatureOfInterest> rdfs:subClassOf [ rdf:type owl:Restriction ;
                                                                owl:onProperty <http://www.w3.org/ns/sosa/hasSample> ;
                                                                owl:allValuesFrom <http://www.w3.org/ns/sosa/Sample>
                                                              ] ,
                                                              [ rdf:type owl:Restriction ;
                                                                owl:onProperty <http://www.w3.org/ns/ssn/hasProperty> ;
                                                                owl:allValuesFrom <http://www.w3.org/ns/ssn/Property>
                                                              ] ,
                                                              [ rdf:type owl:Restriction ;
                                                                owl:onProperty <http://www.w3.org/ns/ssn/hasProperty> ;
                                                                owl:minCardinality "1"^^xsd:nonNegativeInteger
                                                              ] ;
                                              rdfs:isDefinedBy <http://www.w3.org/ns/sosa/> .


###  http://www.w3.org/ns/sosa/ObservableProperty
<http://www.w3.org/ns/sosa/ObservableProperty> rdfs:subClassOf <http://www.w3.org/ns/ssn/Property> ,
                                                               [ rdf:type owl:Restriction ;
                                                                 owl:onProperty <http://www.w3.org/ns/sosa/isObservedBy> ;
                                                                 owl:allValuesFrom <http://www.w3.org/ns/sosa/Sensor>
                                                               ] ,
                                                               [ rdf:type owl:Restriction ;
                                                                 owl:onProperty [ owl:inverseOf <http://www.w3.org/ns/sosa/observedProperty>
                                                                                ] ;
                                                                 owl:allValuesFrom <http://www.w3.org/ns/sosa/Observation>
                                                               ] ,
                                                               [ rdf:type owl:Restriction ;
                                                                 owl:onProperty [ owl:inverseOf <http://www.w3.org/ns/ssn/isProxyFor>
                                                                                ] ;
                                                                 owl:allValuesFrom <http://www.w3.org/ns/ssn/Stimulus>
                                                               ] ;
                                               rdfs:isDefinedBy <http://www.w3.org/ns/sosa/> .


###  http://www.w3.org/ns/sosa/Observation
<http://www.w3.org/ns/sosa/Observation> rdf:type owl:Class ;
                                        rdfs:subClassOf [ rdf:type owl:Restriction ;
                                                          owl:onProperty :hasMedium ;
                                                          owl:allValuesFrom :MediumType
                                                        ] ,
                                                        [ rdf:type owl:Restriction ;
                                                          owl:onProperty :isLocatedIn ;
                                                          owl:allValuesFrom :Location
                                                        ] ,
                                                        [ rdf:type owl:Restriction ;
                                                          owl:onProperty <http://www.w3.org/ns/sosa/hasFeatureOfInterest> ;
                                                          owl:allValuesFrom <http://www.w3.org/ns/sosa/FeatureOfInterest>
                                                        ] ,
                                                        [ rdf:type owl:Restriction ;
                                                          owl:onProperty <http://www.w3.org/ns/sosa/hasResult> ;
                                                          owl:allValuesFrom <http://www.w3.org/ns/sosa/Result>
                                                        ] ,
                                                        [ rdf:type owl:Restriction ;
                                                          owl:onProperty <http://www.w3.org/ns/sosa/madeBySensor> ;
                                                          owl:allValuesFrom <http://www.w3.org/ns/sosa/Sensor>
                                                        ] ,
                                                        [ rdf:type owl:Restriction ;
                                                          owl:onProperty <http://www.w3.org/ns/sosa/observedProperty> ;
                                                          owl:allValuesFrom <http://www.w3.org/ns/sosa/ObservableProperty>
                                                        ] ,
                                                        [ rdf:type owl:Restriction ;
                                                          owl:onProperty <http://www.w3.org/ns/sosa/usedProcedure> ;
                                                          owl:allValuesFrom <http://www.w3.org/ns/sosa/Procedure>
                                                        ] ,
                                                        [ rdf:type owl:Restriction ;
                                                          owl:onProperty <http://www.w3.org/ns/ssn/wasOriginatedBy> ;
                                                          owl:allValuesFrom <http://www.w3.org/ns/ssn/Stimulus>
                                                        ] ,
                                                        [ rdf:type owl:Restriction ;
                                                          owl:onProperty <http://www.w3.org/ns/sosa/hasResult> ;
                                                          owl:minCardinality "1"^^xsd:nonNegativeInteger
                                                        ] ,
                                                        [ rdf:type owl:Restriction ;
                                                          owl:onProperty <http://www.w3.org/ns/sosa/hasFeatureOfInterest> ;
                                                          owl:cardinality "1"^^xsd:nonNegativeInteger
                                                        ] ,
                                                        [ rdf:type owl:Restriction ;
                                                          owl:onProperty <http://www.w3.org/ns/sosa/madeBySensor> ;
                                                          owl:cardinality "1"^^xsd:nonNegativeInteger
                                                        ] ,
                                                        [ rdf:type owl:Restriction ;
                                                          owl:onProperty <http://www.w3.org/ns/sosa/observedProperty> ;
                                                          owl:cardinality "1"^^xsd:nonNegativeInteger
                                                        ] ,
                                                        [ rdf:type owl:Restriction ;
                                                          owl:onProperty <http://www.w3.org/ns/sosa/phenomenonTime> ;
                                                          owl:cardinality "1"^^xsd:nonNegativeInteger
                                                        ] ,
                                                        [ rdf:type owl:Restriction ;
                                                          owl:onProperty <http://www.w3.org/ns/ssn/wasOriginatedBy> ;
                                                          owl:cardinality "1"^^xsd:nonNegativeInteger
                                                        ] ,
                                                        [ rdf:type owl:Restriction ;
                                                          owl:onProperty :accuracy ;
                                                          owl:allValuesFrom xsd:decimal
                                                        ] ,
                                                        [ rdf:type owl:Restriction ;
                                                          owl:onProperty :frequency ;
                                                          owl:allValuesFrom xsd:decimal
                                                        ] ,
                                                        [ rdf:type owl:Restriction ;
                                                          owl:onProperty :latency ;
                                                          owl:allValuesFrom xsd:integer
                                                        ] ,
                                                        [ rdf:type owl:Restriction ;
                                                          owl:onProperty :precision ;
                                                          owl:allValuesFrom xsd:decimal
                                                        ] ,
                                                        [ rdf:type owl:Restriction ;
                                                          owl:onProperty :sensitivity ;
                                                          owl:allValuesFrom xsd:decimal
                                                        ] ,
                                                        [ rdf:type owl:Restriction ;
                                                          owl:onProperty :isAmbient ;
                                                          owl:qualifiedCardinality "1"^^xsd:nonNegativeInteger ;
                                                          owl:onDataRange xsd:boolean
                                                        ] ,
                                                        [ rdf:type owl:Restriction ;
                                                          owl:onProperty :isIndexValue ;
                                                          owl:qualifiedCardinality "1"^^xsd:nonNegativeInteger ;
                                                          owl:onDataRange xsd:boolean
                                                        ] ,
                                                        [ rdf:type owl:Restriction ;
                                                          owl:onProperty :isSetPoint ;
                                                          owl:qualifiedCardinality "1"^^xsd:nonNegativeInteger ;
                                                          owl:onDataRange xsd:boolean
                                                        ] ,
                                                        [ rdf:type owl:Restriction ;
                                                          owl:onProperty :maxValue ;
                                                          owl:qualifiedCardinality "1"^^xsd:nonNegativeInteger ;
                                                          owl:onDataRange xsd:decimal
                                                        ] ,
                                                        [ rdf:type owl:Restriction ;
                                                          owl:onProperty :minValue ;
                                                          owl:qualifiedCardinality "1"^^xsd:nonNegativeInteger ;
                                                          owl:onDataRange xsd:decimal
                                                        ] ,
                                                        [ rdf:type owl:Restriction ;
                                                          owl:onProperty <http://www.w3.org/ns/sosa/resultTime> ;
                                                          owl:cardinality "1"^^xsd:nonNegativeInteger
                                                        ] ;
                                        rdfs:isDefinedBy <http://www.w3.org/ns/sosa/> .


###  http://www.w3.org/ns/sosa/Platform
<http://www.w3.org/ns/sosa/Platform> rdfs:subClassOf [ rdf:type owl:Restriction ;
                                                       owl:onProperty <http://www.w3.org/ns/sosa/hosts> ;
                                                       owl:allValuesFrom <http://www.w3.org/ns/ssn/System>
                                                     ] ,
                                                     [ rdf:type owl:Restriction ;
                                                       owl:onProperty <http://www.w3.org/ns/ssn/inDeployment> ;
                                                       owl:allValuesFrom <http://www.w3.org/ns/ssn/Deployment>
                                                     ] ;
                                     rdfs:isDefinedBy <http://www.w3.org/ns/sosa/> .


###  http://www.w3.org/ns/sosa/Procedure
<http://www.w3.org/ns/sosa/Procedure> rdfs:subClassOf [ rdf:type owl:Restriction ;
                                                        owl:onProperty <http://www.w3.org/ns/ssn/hasInput> ;
                                                        owl:allValuesFrom <http://www.w3.org/ns/ssn/Input>
                                                      ] ,
                                                      [ rdf:type owl:Restriction ;
                                                        owl:onProperty <http://www.w3.org/ns/ssn/hasOutput> ;
                                                        owl:allValuesFrom <http://www.w3.org/ns/ssn/Output>
                                                      ] ,
                                                      [ rdf:type owl:Restriction ;
                                                        owl:onProperty <http://www.w3.org/ns/ssn/implementedBy> ;
                                                        owl:allValuesFrom <http://www.w3.org/ns/ssn/System>
                                                      ] ;
                                      rdfs:isDefinedBy <http://www.w3.org/ns/sosa/> .


###  http://www.w3.org/ns/sosa/Result
<http://www.w3.org/ns/sosa/Result> rdfs:subClassOf [ rdf:type owl:Restriction ;
                                                     owl:onProperty <http://www.w3.org/ns/sosa/isResultOf> ;
                                                     owl:minCardinality "1"^^xsd:nonNegativeInteger
                                                   ] ;
                                   rdfs:isDefinedBy <http://www.w3.org/ns/sosa/> .


###  http://www.w3.org/ns/sosa/Sample
<http://www.w3.org/ns/sosa/Sample> rdfs:subClassOf <http://www.w3.org/ns/sosa/FeatureOfInterest> ,
                                                   <http://www.w3.org/ns/sosa/Result> ,
                                                   [ rdf:type owl:Restriction ;
                                                     owl:onProperty <http://www.w3.org/ns/sosa/isResultOf> ;
                                                     owl:allValuesFrom <http://www.w3.org/ns/sosa/Sampling>
                                                   ] ,
                                                   [ rdf:type owl:Restriction ;
                                                     owl:onProperty <http://www.w3.org/ns/sosa/isSampleOf> ;
                                                     owl:allValuesFrom <http://www.w3.org/ns/sosa/FeatureOfInterest>
                                                   ] ,
                                                   [ rdf:type owl:Restriction ;
                                                     owl:onProperty <http://www.w3.org/ns/sosa/isResultOf> ;
                                                     owl:minCardinality "1"^^xsd:nonNegativeInteger
                                                   ] ,
                                                   [ rdf:type owl:Restriction ;
                                                     owl:onProperty <http://www.w3.org/ns/sosa/isSampleOf> ;
                                                     owl:minCardinality "1"^^xsd:nonNegativeInteger
                                                   ] ;
                                   rdfs:isDefinedBy <http://www.w3.org/ns/sosa/> .


###  http://www.w3.org/ns/sosa/Sampler
<http://www.w3.org/ns/sosa/Sampler> rdfs:subClassOf <http://www.w3.org/ns/ssn/System> ,
                                                    [ rdf:type owl:Restriction ;
                                                      owl:onProperty <http://www.w3.org/ns/sosa/madeSampling> ;
                                                      owl:allValuesFrom <http://www.w3.org/ns/sosa/Sampling>
                                                    ] ,
                                                    [ rdf:type owl:Restriction ;
                                                      owl:onProperty <http://www.w3.org/ns/ssn/implements> ;
                                                      owl:minCardinality "1"^^xsd:nonNegativeInteger
                                                    ] ;
                                    rdfs:isDefinedBy <http://www.w3.org/ns/sosa/> .


###  http://www.w3.org/ns/sosa/Sampling
<http://www.w3.org/ns/sosa/Sampling> rdf:type owl:Class ;
                                     rdfs:subClassOf [ rdf:type owl:Restriction ;
                                                       owl:onProperty <http://www.w3.org/ns/sosa/hasFeatureOfInterest> ;
                                                       owl:allValuesFrom <http://www.w3.org/ns/sosa/FeatureOfInterest>
                                                     ] ,
                                                     [ rdf:type owl:Restriction ;
                                                       owl:onProperty <http://www.w3.org/ns/sosa/hasResult> ;
                                                       owl:allValuesFrom <http://www.w3.org/ns/sosa/Sample>
                                                     ] ,
                                                     [ rdf:type owl:Restriction ;
                                                       owl:onProperty <http://www.w3.org/ns/sosa/madeBySampler> ;
                                                       owl:allValuesFrom <http://www.w3.org/ns/sosa/Sampler>
                                                     ] ,
                                                     [ rdf:type owl:Restriction ;
                                                       owl:onProperty <http://www.w3.org/ns/sosa/usedProcedure> ;
                                                       owl:allValuesFrom <http://www.w3.org/ns/sosa/Procedure>
                                                     ] ,
                                                     [ rdf:type owl:Restriction ;
                                                       owl:onProperty <http://www.w3.org/ns/sosa/hasResult> ;
                                                       owl:minCardinality "1"^^xsd:nonNegativeInteger
                                                     ] ,
                                                     [ rdf:type owl:Restriction ;
                                                       owl:onProperty <http://www.w3.org/ns/sosa/hasFeatureOfInterest> ;
                                                       owl:cardinality "1"^^xsd:nonNegativeInteger
                                                     ] ,
                                                     [ rdf:type owl:Restriction ;
                                                       owl:onProperty <http://www.w3.org/ns/sosa/madeBySampler> ;
                                                       owl:cardinality "1"^^xsd:nonNegativeInteger
                                                     ] ,
                                                     [ rdf:type owl:Restriction ;
                                                       owl:onProperty <http://www.w3.org/ns/sosa/resultTime> ;
                                                       owl:cardinality "1"^^xsd:nonNegativeInteger
                                                     ] ;
                                     rdfs:isDefinedBy <http://www.w3.org/ns/sosa/> .


###  http://www.w3.org/ns/sosa/Sensor
<http://www.w3.org/ns/sosa/Sensor> rdfs:subClassOf <http://www.w3.org/ns/ssn/System> ,
                                                   [ rdf:type owl:Restriction ;
                                                     owl:onProperty :isLocatedIn ;
                                                     owl:allValuesFrom :Location
                                                   ] ,
                                                   [ rdf:type owl:Restriction ;
                                                     owl:onProperty <http://www.w3.org/ns/sosa/madeObservation> ;
                                                     owl:allValuesFrom <http://www.w3.org/ns/sosa/Observation>
                                                   ] ,
                                                   [ rdf:type owl:Restriction ;
                                                     owl:onProperty <http://www.w3.org/ns/sosa/observes> ;
                                                     owl:allValuesFrom <http://www.w3.org/ns/sosa/ObservableProperty>
                                                   ] ,
                                                   [ rdf:type owl:Restriction ;
                                                     owl:onProperty <http://www.w3.org/ns/ssn/detects> ;
                                                     owl:allValuesFrom <http://www.w3.org/ns/ssn/Stimulus>
                                                   ] ,
                                                   [ rdf:type owl:Restriction ;
                                                     owl:onProperty <http://www.w3.org/ns/ssn/implements> ;
                                                     owl:minCardinality "1"^^xsd:nonNegativeInteger
                                                   ] ;
                                   rdfs:isDefinedBy <http://www.w3.org/ns/sosa/> .


###  http://www.w3.org/ns/ssn/Deployment
<http://www.w3.org/ns/ssn/Deployment> rdf:type owl:Class ;
                                      rdfs:subClassOf [ rdf:type owl:Restriction ;
                                                        owl:onProperty <http://www.w3.org/ns/ssn/deployedOnPlatform> ;
                                                        owl:allValuesFrom <http://www.w3.org/ns/sosa/Platform>
                                                      ] ,
                                                      [ rdf:type owl:Restriction ;
                                                        owl:onProperty <http://www.w3.org/ns/ssn/deployedSystem> ;
                                                        owl:allValuesFrom <http://www.w3.org/ns/ssn/System>
                                                      ] ,
                                                      [ rdf:type owl:Restriction ;
                                                        owl:onProperty <http://www.w3.org/ns/ssn/forProperty> ;
                                                        owl:allValuesFrom <http://www.w3.org/ns/ssn/Property>
                                                      ] ;
                                      rdfs:comment "Describes the Deployment of one or more Systems for a particular purpose. Deployment may be done on a Platform."@en ;
                                      rdfs:isDefinedBy <http://www.w3.org/ns/ssn/> ;
                                      rdfs:label "Deployment"@en ;
                                      <http://www.w3.org/2004/02/skos/core#definition> "Describes the Deployment of one or more Systems for a particular purpose. Deployment may be done on a Platform."@en ;
                                      <http://www.w3.org/2004/02/skos/core#example> "For example, a temperature Sensor deployed on a wall, or a whole network of Sensors deployed for an Observation campaign."@en .


###  http://www.w3.org/ns/ssn/Input
<http://www.w3.org/ns/ssn/Input> rdf:type owl:Class ;
                                 rdfs:subClassOf [ rdf:type owl:Restriction ;
                                                   owl:onProperty [ owl:inverseOf <http://www.w3.org/ns/ssn/hasInput>
                                                                  ] ;
                                                   owl:allValuesFrom <http://www.w3.org/ns/sosa/Procedure>
                                                 ] ,
                                                 [ rdf:type owl:Restriction ;
                                                   owl:onProperty [ owl:inverseOf <http://www.w3.org/ns/ssn/hasInput>
                                                                  ] ;
                                                   owl:minCardinality "1"^^xsd:nonNegativeInteger
                                                 ] ;
                                 rdfs:comment "Any information that is provided to a Procedure for its use."@en ;
                                 rdfs:isDefinedBy <http://www.w3.org/ns/ssn/> ;
                                 rdfs:label "Input"@en ;
                                 <http://www.w3.org/2004/02/skos/core#definition> "Any information that is provided to a Procedure for its use."@en .


###  http://www.w3.org/ns/ssn/Output
<http://www.w3.org/ns/ssn/Output> rdf:type owl:Class ;
                                  rdfs:subClassOf [ rdf:type owl:Restriction ;
                                                    owl:onProperty [ owl:inverseOf <http://www.w3.org/ns/ssn/hasOutput>
                                                                   ] ;
                                                    owl:allValuesFrom <http://www.w3.org/ns/sosa/Procedure>
                                                  ] ,
                                                  [ rdf:type owl:Restriction ;
                                                    owl:onProperty [ owl:inverseOf <http://www.w3.org/ns/ssn/hasOutput>
                                                                   ] ;
                                                    owl:minCardinality "1"^^xsd:nonNegativeInteger
                                                  ] ;
                                  rdfs:comment "Any information that is reported from a Procedure."@en ;
                                  rdfs:isDefinedBy <http://www.w3.org/ns/ssn/> ;
                                  rdfs:label "Output"@en ;
                                  <http://www.w3.org/2004/02/skos/core#definition> "Any information that is reported from a Procedure."@en .


###  http://www.w3.org/ns/ssn/Property
<http://www.w3.org/ns/ssn/Property> rdf:type owl:Class ;
                                    rdfs:subClassOf :Property ,
                                                    [ rdf:type owl:Restriction ;
                                                      owl:onProperty <http://www.w3.org/ns/ssn/isPropertyOf> ;
                                                      owl:allValuesFrom <http://www.w3.org/ns/sosa/FeatureOfInterest>
                                                    ] ;
                                    rdfs:comment "A quality of an entity. An aspect of an entity that is intrinsic to and cannot exist without the entity."@en ;
                                    rdfs:isDefinedBy <http://www.w3.org/ns/ssn/> ;
                                    rdfs:label "Property"@en ;
                                    <http://www.w3.org/2004/02/skos/core#definition> "A quality of an entity. An aspect of an entity that is intrinsic to and cannot exist without the entity."@en .


###  http://www.w3.org/ns/ssn/Stimulus
<http://www.w3.org/ns/ssn/Stimulus> rdf:type owl:Class ;
                                    rdfs:subClassOf [ rdf:type owl:Restriction ;
                                                      owl:onProperty <http://www.w3.org/ns/ssn/isProxyFor> ;
                                                      owl:allValuesFrom <http://www.w3.org/ns/sosa/ObservableProperty>
                                                    ] ,
                                                    [ rdf:type owl:Restriction ;
                                                      owl:onProperty [ owl:inverseOf <http://www.w3.org/ns/ssn/detects>
                                                                     ] ;
                                                      owl:allValuesFrom <http://www.w3.org/ns/sosa/Sensor>
                                                    ] ,
                                                    [ rdf:type owl:Restriction ;
                                                      owl:onProperty [ owl:inverseOf <http://www.w3.org/ns/ssn/wasOriginatedBy>
                                                                     ] ;
                                                      owl:allValuesFrom <http://www.w3.org/ns/sosa/Observation>
                                                    ] ;
                                    rdfs:comment "An event in the real world that 'triggers' the Sensor. The properties associated to the Stimulus may be different to the eventual observed ObservableProperty. It is the event, not the object, that triggers the Sensor."@en ;
                                    rdfs:isDefinedBy <http://www.w3.org/ns/ssn/> ;
                                    rdfs:label "Stimulus"@en ;
                                    <http://www.w3.org/2004/02/skos/core#definition> "An event in the real world that 'triggers' the Sensor. The properties associated to the Stimulus may be different to the eventual observed ObservableProperty. It is the event, not the object, that triggers the Sensor."@en .


###  http://www.w3.org/ns/ssn/System
<http://www.w3.org/ns/ssn/System> rdf:type owl:Class ;
                                  rdfs:subClassOf [ rdf:type owl:Restriction ;
                                                    owl:onProperty <http://www.w3.org/ns/sosa/isHostedBy> ;
                                                    owl:allValuesFrom <http://www.w3.org/ns/sosa/Platform>
                                                  ] ,
                                                  [ rdf:type owl:Restriction ;
                                                    owl:onProperty <http://www.w3.org/ns/ssn/hasDeployment> ;
                                                    owl:allValuesFrom <http://www.w3.org/ns/ssn/Deployment>
                                                  ] ,
                                                  [ rdf:type owl:Restriction ;
                                                    owl:onProperty <http://www.w3.org/ns/ssn/hasSubSystem> ;
                                                    owl:allValuesFrom <http://www.w3.org/ns/ssn/System>
                                                  ] ,
                                                  [ rdf:type owl:Restriction ;
                                                    owl:onProperty <http://www.w3.org/ns/ssn/implements> ;
                                                    owl:allValuesFrom <http://www.w3.org/ns/sosa/Procedure>
                                                  ] ,
                                                  [ rdf:type owl:Restriction ;
                                                    owl:onProperty [ owl:inverseOf <http://www.w3.org/ns/ssn/hasSubSystem>
                                                                   ] ;
                                                    owl:allValuesFrom <http://www.w3.org/ns/ssn/System>
                                                  ] ;
                                  rdfs:comment "System is a unit of abstraction for pieces of infrastructure that implement Procedures. A System may have components, its subsystems, which are other systems."@en ;
                                  rdfs:isDefinedBy <http://www.w3.org/ns/ssn/> ;
                                  rdfs:label "System"@en ;
                                  <http://www.w3.org/2004/02/skos/core#definition> "System is a unit of abstraction for pieces of infrastructure that implement Procedures. A System may have components, its subsystems, which are other systems."@en .


###  http://xmlns.com/foaf/0.1/Agent
<http://xmlns.com/foaf/0.1/Agent> rdf:type owl:Class .


#################################################################
#    Individuals
#################################################################

###  http://www.bemserver.org/sensor/xssn/#AIR
:AIR rdf:type owl:NamedIndividual .


###  http://www.bemserver.org/sensor/xssn/#AT_FREQUENCY
:AT_FREQUENCY rdf:type owl:NamedIndividual .


###  http://www.bemserver.org/sensor/xssn/#GAS
:GAS rdf:type owl:NamedIndividual .


###  http://www.bemserver.org/sensor/xssn/#OIL
:OIL rdf:type owl:NamedIndividual .


###  http://www.bemserver.org/sensor/xssn/#ON_VALUE_CHANGE
:ON_VALUE_CHANGE rdf:type owl:NamedIndividual .


###  http://www.bemserver.org/sensor/xssn/#OTHER
:OTHER rdf:type owl:NamedIndividual .


###  http://www.bemserver.org/sensor/xssn/#RADIATION
:RADIATION rdf:type owl:NamedIndividual .


###  http://www.bemserver.org/sensor/xssn/#STEAM
:STEAM rdf:type owl:NamedIndividual .


###  http://www.bemserver.org/sensor/xssn/#WATER
:WATER rdf:type owl:NamedIndividual .


###  http://www.w3.org/ns/ssn/
<http://www.w3.org/ns/ssn/> rdf:type owl:NamedIndividual ,
                                     <http://purl.org/vocommons/voaf#Vocabulary> .


[ rdf:type <http://xmlns.com/foaf/0.1/Agent> ;
  <http://xmlns.com/foaf/0.1/name> "W3C/OGC Spatial Data on the Web Working Group"@en
] .

[ rdf:type <http://xmlns.com/foaf/0.1/Agent> ;
   <http://xmlns.com/foaf/0.1/name> "W3C/OGC Spatial Data on the Web Working Group"@en
 ] .

#################################################################
#    Annotations
#################################################################

<http://www.w3.org/ns/sosa/hasSimpleResult> rdfs:isDefinedBy <http://www.w3.org/ns/sosa/> .


<http://www.w3.org/ns/sosa/isFeatureOfInterestOf> rdfs:isDefinedBy <http://www.w3.org/ns/sosa/> .


###  Generated by the OWL API (version 5.1.14) https://github.com/owlcs/owlapi/
